src/3d/Options.fst
@@ -115,6 +115,10 @@ let emit_output_types_defs : ref bool = alloc true
 
 let emit_smt_encoding : ref bool = alloc false
 
+let z3_test : ref (option vstring) = alloc None
+
+let z3_witnesses : ref (option vstring) = alloc None
+
 noeq
 type cmd_option_kind =
   | OptBool:
@@ -347,6 +351,8 @@ let (display_usage_2, compute_options_2, fstar_options) =
     CmdOption "skip_o_rules" (OptBool skip_o_rules) "With --makefile, do not generate rules for .o files" [];
     CmdFStarOption (let open FStar.Getopt in noshort, "version", ZeroArgs (fun _ -> FStar.IO.print_string (Printf.sprintf "EverParse/3d %s\nCopyright 2018, 2019, 2020 Microsoft Corporation\n" Version.everparse_version); exit 0), "Show this version of EverParse");
     CmdOption "equate_types" (OptList "an argument of the form A,B, to generate asserts of the form (A.t == B.t)" valid_equate_types equate_types_list) "Takes an argument of the form A,B and then for each entrypoint definition in B, it generates an assert (A.t == B.t) in the B.Types file, useful when refactoring specs, you can provide multiple equate_types on the command line" [];
+    CmdOption "z3_test" (OptStringOption "parser name" always_valid z3_test) "produce positive and negative test cases for a given parser" [];
+    CmdOption "z3_witnesses" (OptStringOption "nb" always_valid z3_witnesses) "ask for nb distinct test witnesses" [];
     CmdOption "__arg0" (OptStringOption "executable name" always_valid arg0) "executable name to use for the help message" [];
     CmdOption "__micro_step" (OptStringOption "verify|extract|copy_clang_format|emit_config" valid_micro_step micro_step) "micro step" [];
     CmdOption "__produce_c_from_existing_krml" (OptBool produce_c_from_existing_krml) "produce C from .krml files" [];
@@ -511,3 +517,14 @@ let config_module_name () =
 
 let get_emit_smt_encoding () =
   !emit_smt_encoding
+
+let get_z3_test () = !z3_test
+
+let get_z3_witnesses () =
+  match !z3_witnesses with
+  | None -> 1
+  | Some s ->
+  try
+    let n = OS.int_of_string s in
+    if n < 1 then 1 else n
+  with _ -> 1
