src/3d/OS.fsti
@@ -20,3 +20,7 @@ val extension: string -> Tot string
 val file_exists: string -> FStar.All.ML bool
 
 val file_contents: string -> FStar.All.ML string
+
+(* Moved here to break dependency cycle *)
+
+val int_of_string (x:string) : FStar.All.ML int
