src/3d/Options.fsti
@@ -63,3 +63,7 @@ val make_includes : unit -> ML string
 val config_module_name : unit -> ML (option string)
 
 val get_emit_smt_encoding: unit -> ML bool
+
+val get_z3_test: unit -> ML (option string)
+
+val get_z3_witnesses: unit -> ML int
